update

PoL/Consensus/ProtocolC/ConsistencyC.lean
@@ -1,7 +1,7 @@
 import PoL.Consensus.ProtocolC.StateC
 
 def protocolC_step_with_crash
-  (state : StateC) (new_block : Block) (current_view : ℕ) (is_leader_crashed: ℕ → Bool) (next_leader: StateC → ℕ) : StateC :=
+  (state : StateC) (new_block : Block) (current_view : ℕ) (is_leader_crashed: ℕ → Bool) (is_crashed: ℕ → Bool) (next_leader: StateC → ℕ) : StateC :=
   let n := state.validators.length
 
   -- Phase 1: Collect known chains with views from non-crashed validators
@@ -26,12 +26,12 @@ def protocolC_step_with_crash
         if has_write_quorum ack_count n then
           { finalized_chain := new_chain_with_view.chain,
             known_chain := new_chain_with_view,
-            crashed := v.crashed,
+            crashed := v.crashed ∨ is_crashed v.id,
             id := v.id }
         else
           { finalized_chain := v.finalized_chain,
             known_chain := new_chain_with_view,
-            crashed := v.crashed,
+            crashed := v.crashed ∨ is_crashed v.id,
             id := v.id }
       | none => v
     else v)
@@ -41,9 +41,19 @@ def protocolC_step_with_crash
 
 def protocolC_evolve
   (initial_state : StateC) (blocks : ℕ → Block)
-  (is_leader_crashed_at_t: ℕ → ℕ → Bool) (next_leader_at_t: ℕ → StateC → ℕ)
+  (is_leader_crashed_at_t: ℕ → ℕ → Bool) (is_crashed_at_t: ℕ → ℕ → Bool) (next_leader_at_t: ℕ → StateC → ℕ)
   : ℕ → StateC
   | 0   => initial_state
   | t+1 => protocolC_step_with_crash
-            (protocolC_evolve initial_state blocks is_leader_crashed_at_t next_leader_at_t t)
-            (blocks t) t (is_leader_crashed_at_t t) (next_leader_at_t t)
+            (protocolC_evolve initial_state blocks is_leader_crashed_at_t is_crashed_at_t next_leader_at_t t)
+            (blocks t) t (is_leader_crashed_at_t t) (is_crashed_at_t t) (next_leader_at_t t)
+
+theorem protocolC_consistency
+    (initial_state : StateC)
+    (blocks : ℕ → Block)
+    (is_leader_crashed_at_t: ℕ → ℕ → Bool)
+    (is_crashed_at_t: ℕ → ℕ → Bool)
+    (h_initial_consistent : StateCIsConsistent initial_state)
+    (next_leader_at_t: ℕ → StateC → ℕ) :
+    ∀ t, StateCIsConsistent (protocolC_evolve initial_state blocks is_leader_crashed_at_t is_crashed_at_t next_leader_at_t t) := by
+    sorry
